ulib/ml/FStar_Pervasives_Native.ml
@@ -156,6 +156,7 @@ type norm_step =
     | NBE
     | UnfoldOnly : string list -> norm_step
     | UnfoldFully : string list -> norm_step
+    | UnfoldAttr : 'a -> norm_step
 
 let simplify : norm_step = Simpl
 let weak    : norm_step = Weak
@@ -166,6 +167,7 @@ let zeta    : norm_step = Zeta
 let iota    : norm_step = Iota
 let delta_only (s:string list) : norm_step = UnfoldOnly s
 let delta_fully (s:string list) : norm_step = UnfoldFully s
+let delta_attr a = UnfoldAttr a
 let reify   : norm_step = Reify
 let nbe     : norm_step = NBE
 
